src/arch/x64/X64.Vale.StrongPost_i.fst
@@ -5,15 +5,7 @@ open X64.Vale.Decls
 
 #reset-options "--initial_fuel 1 --max_fuel 1 --initial_ifuel 1 --max_ifuel 1 --z3rlimit 20"
 
-// REVIEW: Hide polymorphic Map functions behind monomorphic functions
-// until we have a better way to prevent the nat64 type argument from getting normalized
-let mem_contains m i = Map.contains m i
-let mem_sel m i = Map.sel m i
-let mem_upd m i n = Map.upd m i n
-
-let lemma_mem_contains m i = ()
-let lemma_mem_sel m i = ()
-let lemma_mem_upd m i n = ()
+let empty = ()
 
 let rec lemma_regs_match_self (regs:list reg) (s:state) : Lemma
   (requires True)
@@ -27,155 +19,145 @@ let lemma_update_reg_equal (r:reg) (v:nat64) (s1:state) (s2:state) : Lemma
   (ensures ((update_reg r v s1).regs == s2.regs)) =
   ()
 
-let lemma_strong_post_ins (i:ins) (inss:list ins) (s0:state) (sN:state) : Ghost (option state)
-  (requires
-    Some sN == va_eval_code (va_Block (inss_to_codes (i::inss))) s0 /\
-    s0.ok)
-  (ensures (fun sM ->
-    match sM with
-    | None -> strong_post (i::inss) s0 sN
-    | Some sM ->
-        Some sN == va_eval_code (va_Block (inss_to_codes inss)) sM /\
-        sM.ok /\
-        (strong_post inss sM sN ==> strong_post (i::inss) s0 sN))) =
+let assert_from_norm' (p:Type0): Lemma
+  (requires (Prims.norm [delta_only wp_code_delta; zeta; iota; primops] p))
+  (ensures p)
+  = ()
+
+let assert_to_norm' (p:Type0): Lemma
+  (requires p)
+  (ensures (Prims.norm [delta_only wp_code_delta; zeta; iota; primops] p))
+  = ()
+
+let lemma_weak_pre_ins (i:ins) (inss:list ins) 
+			       (s0:state) (sN:state) (post: unit -> Type) :
+  Ghost (option state)
+         (requires (s0.ok /\
+		    Some sN == va_eval_code (va_Block (inss_to_codes (i::inss))) s0) /\
+		    wp_code (i::inss) (augment sN post) s0)
+	 (ensures (fun sM ->
+		     match sM with
+		     | None -> False
+		     | Some sM ->
+			    Some sN == va_eval_code (va_Block (inss_to_codes inss)) sM /\
+			    sM.ok /\
+			    wp_code inss (augment sN post) sM)) =
   let b0 = inss_to_codes (i::inss) in
-  let none_post () : Ghost (option state)
-    (requires normalize (strong_post (i::inss) s0 sN))
-    (ensures fun _ -> strong_post (i::inss) s0 sN) =
-    assert_norm (strong_post (i::inss) s0 sN);
-    None
-    in
-  let some_post_helper (sM:state) (p:Type0) : Ghost (option state)
-    (requires strong_post inss sM sN ==> normalize p)
-    (ensures fun _ -> strong_post inss sM sN ==> p) =
+  (* this results in:
+   Not an embedded list: X64.Vale.StrongPost_i.wp_code_delta")
+  let some_pre (sM:state) (p:Type0) : Ghost (option state)
+    (requires p)
+    (ensures fun _ -> Prims.norm [delta_only wp_code_delta; zeta; iota; primops] p) =
+    assert_to_norm' p;
     Some sM
-    in
-  let some_post (sM:state) : Ghost (option state)
-    (requires strong_post inss sM sN ==> normalize (strong_post (i::inss) s0 sN))
-    (ensures fun _ -> strong_post inss sM sN ==> strong_post (i::inss) s0 sN) =
-    some_post_helper sM (strong_post (i::inss) s0 sN)
-    in
+  in*)
+  let _ = assert_to_norm'(wp_code (i::inss) (augment sN post) s0) in
   match i with
   | Mov64 (OReg dst) src ->
       if dst <> Rsp && valid_operand_norm src s0 then
         let (bM, sM) = va_lemma_Mov64 b0 s0 sN (OReg dst) src in
-        some_post sM
-      else none_post ()
+	  Some sM
+      else 
+	  None
   | Load64 (OReg dst) (OReg src) offset ->
       if dst <> Rsp && valid_src_addr s0.mem (s0.regs src + offset) then
         let (bM, sM) = va_lemma_Load64 b0 s0 sN (OReg dst) (OReg src) offset in
-        some_post sM
-      else none_post ()
+  	  Some sM
+      else
+  	  None
   | Store64 (OReg dst) src offset ->
       if valid_dst_addr s0.mem (s0.regs dst + offset) && valid_operand_norm src s0 then
         let (bM, sM) = va_lemma_Store64 b0 s0 sN (OReg dst) src offset in
-        some_post sM
-      else none_post ()
+  	  Some sM
+      else
+  	  None
   | Add64Wrap (OReg dst) src ->
       if dst <> Rsp && valid_operand_norm src s0 then
         let (bM, sM) = va_lemma_Add64Wrap b0 s0 sN (OReg dst) src in
-        some_post sM
-      else none_post ()
+  	  Some sM
+      else
+  	  None
   | Adc64Wrap (OReg dst) src ->
       if dst <> Rsp && valid_operand_norm src s0 then
         let (bM, sM) = va_lemma_Adc64Wrap b0 s0 sN (OReg dst) src in
-        some_post sM
-      else none_post ()
+  	  Some sM
+      else
+  	  None
   | Mul64Wrap src ->
       if valid_operand_norm src s0 then
         let (bM, sM) = va_lemma_Mul64Wrap b0 s0 sN src in
-        some_post sM
-      else none_post ()
+  	  Some sM
+      else
+  	  None
   | IMul64 (OReg dst) src ->
       let a = s0.regs dst `op_Multiply` eval_operand_norm src s0 in
       if dst <> Rsp && valid_operand_norm src s0 && a < nat64_max then
         let (bM, sM) = va_lemma_IMul64 b0 s0 sN (OReg dst) src in
-        some_post sM
-      else none_post ()
+  	  Some sM
+      else
+  	  None
   | And64 (OReg dst) src ->
     let a = logand64 (s0.regs dst) (eval_operand_norm src s0) in
     if dst <> Rsp && valid_operand_norm src s0 then
       let (bM, sM) = va_lemma_And64 b0 s0 sN (OReg dst) src in
-      some_post sM
-    else none_post ()
+  	  Some sM
+      else
+  	  None
   | Shr64 (OReg dst) src ->
     let a = shift_right64 (s0.regs dst) (eval_operand_norm src s0) in
     if dst <> Rsp && valid_operand_norm src s0 then
       let (bM, sM) = va_lemma_Shr64 b0 s0 sN (OReg dst) src in
-      some_post sM
-    else none_post ()
+  	  Some sM
+      else
+  	  None
   | Sub64 (OReg dst) src ->
-    if dst <> Rsp && valid_operand_norm src s0 && 0 <= (s0.regs dst) - (eval_operand_norm src s0) then
+    if dst <> Rsp && valid_operand_norm src s0 && 0 <= 
+		    (s0.regs dst) - (eval_operand_norm src s0) then
       let (bM, sM) = va_lemma_Sub64 b0 s0 sN (OReg dst) src in
-      some_post sM
-    else none_post ()
-  | _ -> assume false; None
+  	  Some sM
+      else
+  	  None
+  | _ -> None
 
-let rec lemma_strong_post (inss:list ins) (s0:state) (sN:state) : Lemma
+
+ let rec lemma_weak_pre (inss:list ins) (s0:state) (sN:state) (post: unit -> Type0) : Lemma
   (requires
     Some sN == va_eval_code (va_Block (inss_to_codes inss)) s0 /\
-    s0.ok)
+    s0.ok /\
+    wp_code inss (augment sN post) s0)
   (ensures
-    strong_post inss s0 sN) =
+    post ())
+   =
   match inss with
   | [] ->
       let _ = va_lemma_empty s0 sN in
-      let regs = [Rax; Rbx; Rcx; Rdx; Rsi; Rdi; Rbp; Rsp; R8; R9; R10; R11; R12; R13; R14; R15] in
+      let regs = [Rax; Rbx; Rcx; Rdx; Rsi; Rdi; Rbp; 
+		  Rsp; R8; R9; R10; R11; R12; R13; R14; R15] in
       lemma_regs_match_self regs s0;
-      assert_norm (strong_post inss s0 sN);
+      assert_to_norm'(wp_code [] (augment sN post) s0);
       ()
   | i::inss ->
-    (
-      match lemma_strong_post_ins i inss s0 sN with
-      | None -> ()
-      | Some sM -> lemma_strong_post inss sM sN
+    ( 
+      match lemma_weak_pre_ins i inss s0 sN post with
+      | None -> assert(post ())
+      | Some sM -> lemma_weak_pre inss sM sN post
     )
 
-let assert_to_norm (p:Type0) : Lemma
-  (requires p)
-  (ensures (normalize p))
-  = ()
+let lemma_weakest_pre_norm' (inss: list ins) (s0: state) (sN:state) (#post:unit -> Type0) :
+  Lemma (requires
+	  (forall ok0 regs0 flags0 mem0.
+     	    ok0 == s0.ok /\
+     	    regs0 == s0.regs /\
+     	    flags0 == s0.flags /\
+     	    mem0 == s0.mem ==>
+	    s0.ok /\
+	    Some sN == va_eval_code (va_Block (normalize_term (inss_to_codes inss))) s0 /\
+	    Prims.norm [delta_only wp_code_delta; zeta; iota; primops]
+		       (wp_code (normalize_term inss) (augment sN post)
+				   ({ok=ok0; regs=regs0; flags=flags0; mem=mem0}))))
+	(ensures (post ())) = 
+  assert_from_norm' (wp_code inss (augment sN post) s0);
+  lemma_weak_pre inss s0 sN post
 
-let va_lemma_strong_post_norm inss s0 sN =
-  lemma_strong_post inss s0 sN;
-  assert_to_norm (strong_post inss s0 sN);
-  ()
-
-
-
-let rec lemma_weak_pre (inss:list ins) (s0:state) (post: state -> Type) (sN:state) : Lemma
-  (requires
-    Some sN == va_eval_code (va_Block (inss_to_codes inss)) s0 /\
-    s0.ok)
-  (ensures
-    wp_code inss (fun sN' -> sN' == sN ==> post sN') s0) =
-  match inss with
-  | [] ->
-      let _ = va_lemma_empty s0 sN in
-      let regs = [Rax; Rbx; Rcx; Rdx; Rsi; Rdi; Rbp; Rsp; R8; R9; R10; R11; R12; R13; R14; R15] in
-      lemma_regs_match_self regs s0;
-      assert_norm (wp_code inss s0 (fun sN' -> sN' == sN ==> post sN'));
-      ()
-  | i::inss ->
-    (
-      match lemma_strong_post_ins i inss s0 sN with
-      | None -> ()
-      | Some sM -> lemma_strong_post inss sM sN
-    )
-
-assume val lemma_weak_pre_ins: (i:ins) -> (inss:list ins) -> 
-			       (s0:state) -> (sN:state) ->
-			       (post: state -> Type) -> 
-  Ghost (state -> Type)
-         (requires (s0.ok /\
-		    Some sN == va_eval_code (va_Block (inss_to_codes (i::inss))) s0))
-	 (ensures (fun post' ->
-		     match sM with
-		     | None -> wp_code (i::inss) (fun sN' -> sN' == sM ==> post sN') s0
-		     | Some sM ->
-			    Some sN == va_eval_code (va_Block (inss_to_codes inss)) sM /\
-			    sM.ok /\
-			    wp
-		    
-
-let lemma_weakest_pre_norm inss s0 = admit ()
+let va_lemma_weakest_pre_norm inss s0 sN =
+  admit () // connect with proof above
