src/arch/x64/X64.Vale.StrongPost_i.fsti
@@ -5,21 +5,7 @@ open X64.Vale.Decls
 
 #reset-options "--z3rlimit 20"
 
-val mem_contains : m:mem -> i:int -> bool
-val mem_sel : m:mem -> i:int -> nat64
-val mem_upd : m:mem -> i:int -> n:nat64 -> mem
-
-val lemma_mem_contains : m:mem -> i:int -> Lemma
-  (ensures mem_contains m i == Map.contains m i)
-  [SMTPat (mem_contains m i)]
-
-val lemma_mem_sel : m:mem -> i:int -> Lemma
-  (ensures mem_sel m i == Map.sel m i)
-  [SMTPat (mem_sel m i)]
-
-val lemma_mem_upd : m:mem -> i:int -> n:nat64 -> Lemma
-  (ensures mem_upd m i n == Map.upd m i n)
-  [SMTPat (mem_upd m i n)]
+val empty : unit //annoying
 
 type ins =
   | Mov64 : dst:va_operand -> src:va_operand -> ins
@@ -47,7 +33,7 @@ unfold let va_fast_ins_Sub64 = Sub64
 unfold let va_inss = list ins
 
 let valid_maddr_norm (m:maddr) (s:state) : bool =
-  mem_contains s.mem (eval_maddr m s)
+  Map.contains s.mem (eval_maddr m s)
 
 let valid_operand_norm (o:operand) (s:state) : bool =
   match o with
@@ -59,7 +45,7 @@ let eval_operand_norm (o:operand) (s:state) : nat64 =
   match o with
   | OConst n -> if 0 <= n && n < nat64_max then n else 0
   | OReg r -> s.regs r
-  | OMem m -> mem_sel s.mem (eval_maddr m s)
+  | OMem m -> Map.sel s.mem (eval_maddr m s)
 
 let rec regs_match (regs:list reg) (s0:state) (s1:state) =
   match regs with
@@ -67,99 +53,25 @@ let rec regs_match (regs:list reg) (s0:state) (s1:state) =
   | r::regs -> s0.regs r == s1.regs r /\ regs_match regs s0 s1
 
 let all_regs_match (s0:state) (s1:state) =
-  let regs = [Rax; Rbx; Rcx; Rdx; Rsi; Rdi; Rbp; Rsp; R8; R9; R10; R11; R12; R13; R14; R15] in
+  let regs = [Rax; Rbx; Rcx; Rdx; Rsi; Rdi; Rbp; Rsp; R8; 
+	      R9; R10; R11; R12; R13; R14; R15] in
   regs_match regs s0 s1
-
-[@"opaque_to_smt"] // because of exists-interp axiom, avoid giving this to SMT
-let rec strong_post (inss:list ins) (s0:state) (sN:state) : Type0 =
-  match inss with
-  | [] ->
-      sN.ok /\
-      sN.flags == s0.flags /\
-      sN.mem == s0.mem /\
-      all_regs_match s0 sN // for efficiency, we apply s0.regs to all registers and then discard s0.regs
-  | (Mov64 (OReg Rsp) _)::_ -> True
-  | (Mov64 (OReg dst) src)::inss ->
-      not (valid_operand_norm src s0) \/
-      (exists x.
-        x == eval_operand_norm src s0 /\
-        strong_post inss (update_reg dst x s0) sN)
-  | (Load64 (OReg Rsp) _ _)::_ -> True
-  | (Load64 (OReg dst) (OReg src) offset)::inss ->
-      not (mem_contains s0.mem (s0.regs src + offset)) \/
-      (exists x.
-        x == mem_sel s0.mem (s0.regs src + offset) /\
-        strong_post inss (update_reg dst x s0) sN)
-  | (Store64 (OReg dst) src offset)::inss ->
-      not (valid_operand_norm src s0) \/
-      not (mem_contains s0.mem (s0.regs dst + offset)) \/
-      (exists x.
-        x == mem_upd s0.mem (s0.regs dst + offset) (eval_operand_norm src s0) /\
-        strong_post inss ({s0 with mem = x}) sN)
-  | (Add64Wrap (OReg Rsp) _)::_ -> True
-  | (Add64Wrap (OReg dst) src)::inss ->
-      not (valid_operand_norm src s0) \/
-      (exists a x (f:nat64).
-        a == s0.regs dst + eval_operand_norm src s0 /\
-        x == (if a < nat64_max then a else a - nat64_max) /\
-        cf f == (a >= nat64_max) /\
-        strong_post inss ({update_reg dst x s0 with flags = f}) sN)
-  | (Adc64Wrap (OReg Rsp) _)::_ -> True
-  | (Adc64Wrap (OReg dst) src)::inss ->
-      not (valid_operand_norm src s0) \/
-      (exists a x (f:nat64).
-        a == s0.regs dst + eval_operand_norm src s0 + (if cf s0.flags then 1 else 0) /\
-        x == (if a < nat64_max then a else a - nat64_max) /\
-        cf f == (a >= nat64_max) /\
-        strong_post inss ({update_reg dst x s0 with flags = f}) sN)
-  | (Mul64Wrap src)::inss ->
-      not (valid_operand_norm src s0) \/
-      (exists (rax:nat64) (rdx:nat64) (f:nat64).
-        nat64_max `op_Multiply` rdx + rax == s0.regs Rax `op_Multiply` eval_operand_norm src s0 /\
-        strong_post inss (update_reg Rdx rdx (update_reg Rax rax ({s0 with flags = f}))) sN)
-  | (IMul64 (OReg Rsp) _)::_ -> True
-  | (IMul64 (OReg dst) src)::inss ->
-      let a = s0.regs dst `op_Multiply` eval_operand_norm src s0 in
-      not (valid_operand_norm src s0) \/
-      not (a < nat64_max) \/
-      (exists (x:nat64) (f:nat64).
-        x == a /\
-        strong_post inss ({update_reg dst x s0 with flags = f}) sN)
-  | (And64 (OReg Rsp) _)::_ -> True
-  | (And64 (OReg dst) src)::inss ->
-    let a = logand64 (s0.regs dst) (eval_operand_norm src s0) in
-    not (valid_operand_norm src s0) \/
-    (exists (x:nat64) (f:nat64).
-      x == a /\
-      strong_post inss ({update_reg dst x s0 with flags = f}) sN)
-  | (Shr64 (OReg Rsp) _)::_ -> True
-  | (Shr64 (OReg dst) src)::inss ->
-    let a = shift_right64 (s0.regs dst) (eval_operand_norm src s0) in
-    not (valid_operand_norm src s0) \/
-    (exists (x:nat64) (f:nat64).
-      x == a /\
-      strong_post inss ({update_reg dst x s0 with flags = f}) sN)
-  | (Sub64 (OReg Rsp) _)::_ -> True
-  | (Sub64 (OReg dst) src)::inss ->
-      not (valid_operand_norm src s0) \/
-      not (0 <= s0.regs dst - eval_operand_norm src s0) \/
-      (exists a x (f:nat64).
-        a == s0.regs dst - eval_operand_norm src s0 /\
-        x == a /\
-        strong_post inss ({update_reg dst x s0 with flags = f}) sN)
-  | _ -> True
 
 let rec inss_to_codes (inss:list ins) : list va_code =
   match inss with
   | (Mov64 (OReg Rsp) _)::inss -> []
   | (Mov64 (OReg dst) src)::inss -> (va_code_Mov64 (OReg dst) src)::(inss_to_codes inss)
   | (Load64 (OReg Rsp) _ _)::inss -> []
-  | (Load64 (OReg dst) (OReg src) offset)::inss -> (va_code_Load64 (OReg dst) (OReg src) offset)::(inss_to_codes inss)
-  | (Store64 (OReg dst) src offset)::inss -> (va_code_Store64 (OReg dst) src offset)::(inss_to_codes inss)
+  | (Load64 (OReg dst) (OReg src) offset)::inss ->
+    (va_code_Load64 (OReg dst) (OReg src) offset)::(inss_to_codes inss)
+  | (Store64 (OReg dst) src offset)::inss -> 
+    (va_code_Store64 (OReg dst) src offset)::(inss_to_codes inss)
   | (Add64Wrap (OReg Rsp) _)::inss -> []
-  | (Add64Wrap (OReg dst) src)::inss -> (va_code_Add64Wrap (OReg dst) src)::(inss_to_codes inss)
+  | (Add64Wrap (OReg dst) src)::inss -> 
+    (va_code_Add64Wrap (OReg dst) src)::(inss_to_codes inss)
   | (Adc64Wrap (OReg Rsp) _)::inss -> []
-  | (Adc64Wrap (OReg dst) src)::inss -> (va_code_Adc64Wrap (OReg dst) src)::(inss_to_codes inss)
+  | (Adc64Wrap (OReg dst) src)::inss -> 
+    (va_code_Adc64Wrap (OReg dst) src)::(inss_to_codes inss)
   | (Mul64Wrap src)::inss -> (va_code_Mul64Wrap src)::(inss_to_codes inss)
   | (IMul64 (OReg Rsp) _)::inss -> []
   | (IMul64 (OReg dst) src)::inss -> (va_code_IMul64 (OReg dst) src)::(inss_to_codes inss)
@@ -171,8 +83,11 @@ let rec inss_to_codes (inss:list ins) : list va_code =
   | (Sub64 (OReg dst) src)::inss -> (va_code_Sub64 (OReg dst) src)::(inss_to_codes inss)
   | _ -> []
 
+let augment (st : state) (post: unit -> Type0) (final_state: state) : Type0 =
+ final_state == st ==> post ()
+
 [@"opaque_to_smt"]
-let rec wp_code (inss : list ins) (post: state -> Type0) (s0:state): Type0 =
+let rec wp_code (inss : list ins) (post: state -> Type0) (s0:state) : Type0 =
   match inss with
   | [] ->
        (forall okN regsN flagsN memN.
@@ -189,30 +104,68 @@ let rec wp_code (inss : list ins) (post: state -> Type0) (s0:state): Type0 =
           wp_code inss post (update_reg dst x s0))
   | (Load64 (OReg Rsp) _ _) :: inss -> False
   | (Load64 (OReg dst) (OReg src) offset) :: inss ->
-    mem_contains s0.mem (s0.regs src + offset) /\
-    (forall x. x == mem_sel s0.mem (s0.regs src + offset) ==>
+    Map.contains s0.mem (s0.regs src + offset) /\
+    (forall x. x == Map.sel s0.mem (s0.regs src + offset) ==>
           wp_code inss post (update_reg dst x s0))
   | (Store64 (OReg dst) src offset) :: inss ->
     (valid_operand_norm src s0) /\
-    (mem_contains s0.mem (s0.regs dst + offset)) /\
+    (Map.contains s0.mem (s0.regs dst + offset)) /\
     (forall x.
-       x == mem_upd s0.mem (s0.regs dst + offset) (eval_operand_norm src s0) ==>
+       x == Map.upd s0.mem (s0.regs dst + offset) (eval_operand_norm src s0) ==>
        wp_code inss post ({s0 with mem = x}))
-  | _ -> True
-
-
-val va_lemma_strong_post_norm : inss:list ins -> s0:state -> sN:state -> Lemma
-  (requires
-    Some sN == va_eval_code (va_Block (normalize_term (inss_to_codes inss))) s0 /\
-    s0.ok)
-  (ensures
-    exists ok0 regs0 flags0 mem0 okN regsN flagsN memN.
-      {:pattern ({ok = ok0; regs = regs0; flags = flags0; mem = mem0}); ({ok = okN; regs = regsN; flags = flagsN; mem = memN})}
-      ok0 == s0.ok /\ regs0 == s0.regs /\ flags0 == s0.flags /\ mem0 == s0.mem /\
-      okN == sN.ok /\ regsN == sN.regs /\ flagsN == sN.flags /\ memN == sN.mem /\
-      normalize (strong_post inss
-        ({ok = ok0; regs = regs0; flags = flags0; mem = mem0})
-        ({ok = okN; regs = regsN; flags = flagsN; mem = memN})))
+  | (Add64Wrap (OReg Rsp) _)::_ -> False
+  | (Add64Wrap (OReg dst) src)::inss ->
+      (valid_operand_norm src s0) /\
+      (forall a x (f:nat64).
+        a == s0.regs dst + eval_operand_norm src s0 /\
+        x == (if a < nat64_max then a else a - nat64_max) /\
+        cf f == (a >= nat64_max) ==>
+        wp_code inss post ({update_reg dst x s0 with flags = f}))
+  | (Adc64Wrap (OReg Rsp) _)::_ -> False
+  | (Adc64Wrap (OReg dst) src)::inss ->
+      (valid_operand_norm src s0) /\
+      (forall a x (f:nat64).
+        a == s0.regs dst + eval_operand_norm src s0 + (if cf s0.flags then 1 else 0) /\
+        x == (if a < nat64_max then a else a - nat64_max) /\
+        cf f == (a >= nat64_max) ==>
+        wp_code inss post ({update_reg dst x s0 with flags = f}))
+  | (Mul64Wrap src)::inss ->
+      (valid_operand_norm src s0) /\
+      (forall (rax:nat64) (rdx:nat64) (f:nat64).
+        nat64_max `op_Multiply` rdx + rax == 
+		  s0.regs Rax `op_Multiply` eval_operand_norm src s0 ==>
+        wp_code inss post (update_reg Rdx rdx (update_reg Rax rax ({s0 with flags = f}))))
+  | (IMul64 (OReg Rsp) _)::_ -> False
+  | (IMul64 (OReg dst) src)::inss ->
+      let a = s0.regs dst `op_Multiply` eval_operand_norm src s0 in
+      (valid_operand_norm src s0) /\
+      (a < nat64_max) /\
+      (forall (x:nat64) (f:nat64).
+        x == a ==>
+        wp_code inss post ({update_reg dst x s0 with flags = f}))
+  | (And64 (OReg Rsp) _)::_ -> False
+  | (And64 (OReg dst) src)::inss ->
+    let a = logand64 (s0.regs dst) (eval_operand_norm src s0) in
+    (valid_operand_norm src s0) /\
+    (forall (x:nat64) (f:nat64).
+      x == a ==>
+      wp_code inss post ({update_reg dst x s0 with flags = f}))
+  | (Shr64 (OReg Rsp) _)::_ -> False
+  | (Shr64 (OReg dst) src)::inss ->
+    let a = shift_right64 (s0.regs dst) (eval_operand_norm src s0) in
+    (valid_operand_norm src s0) /\
+    (forall (x:nat64) (f:nat64).
+      x == a ==>
+      wp_code inss post ({update_reg dst x s0 with flags = f}))
+  | (Sub64 (OReg Rsp) _)::_ -> False
+  | (Sub64 (OReg dst) src)::inss ->
+      (valid_operand_norm src s0) /\
+      (0 <= s0.regs dst - eval_operand_norm src s0) /\
+      (forall a x (f:nat64).
+        a == s0.regs dst - eval_operand_norm src s0 /\
+        x == a ==>
+        wp_code inss post ({update_reg dst x s0 with flags = f}))
+  | _ -> False
 
 let wp_code_delta = [
   "X64.Vale.StrongPost_i.wp_code";
@@ -225,11 +178,13 @@ let wp_code_delta = [
   "X64.Vale.State_i.__proj__Mkstate__item__ok" ;
   "X64.Vale.State_i.__proj__Mkstate__item__flags";
   "X64.Vale.State_i.__proj__Mkstate__item__mem";
-  "X64.Vale.StrongPost_i.valid_operand_norm"
+  "X64.Vale.StrongPost_i.valid_operand_norm";
+  "X64.Vale.StrongPost_i.augment"
   ]
 
+
 [@"uninterpreted_by_smt"]
-val lemma_weakest_pre_norm: inss:list ins -> s0:state -> sN:state -> PURE unit
+val va_lemma_weakest_pre_norm (inss:list ins) (s0:state) (sN:state) : PURE unit
   (fun (post:(unit -> Type)) ->
      forall ok0 regs0 flags0 mem0.
         ok0 == s0.ok /\
@@ -239,15 +194,15 @@ val lemma_weakest_pre_norm: inss:list ins -> s0:state -> sN:state -> PURE unit
         s0.ok /\
         Some sN == va_eval_code (va_Block (normalize_term (inss_to_codes inss))) s0 /\
         Prims.norm [delta_only wp_code_delta; zeta; iota; primops]
-                   (wp_code inss
-                            (fun final_state -> final_state==sN ==> post ())
+                   (wp_code (normalize_term inss) (augment sN post)
                      ({ok=ok0; regs=regs0; flags=flags0; mem=mem0})))
+		     
 
 (* #reset-options "--log_queries --debug X64.Vale.StrongPost_i --debug_level print_normalized_terms" *)
 (* let test_lemma (s0:state) = *)
 (*     assume (s0.ok); *)
-(*     assume (mem_contains s0.mem (s0.regs Rsi)); *)
-(*     assume (mem_contains s0.mem (s0.regs Rcx)); *)
+(*     assume (Map.contains s0.mem (s0.regs Rsi)); *)
+(*     assume (Map.contains s0.mem (s0.regs Rcx)); *)
 (*     let i1 = Prims.set_range_of (Load64 (OReg Rax) (OReg Rsi) 0) *)
 (*                                 (mk_range "load-instruction-1" 1 1 2 0) in *)
 (*     let i2 = Prims.set_range_of (Load64 (OReg Rbx) (OReg Rcx) 0) *)
